Wavelet/HighLevel.lean
@@ -58,6 +58,26 @@ abbrev Dataflow.Proc.semanticsᵢ
     Semantics.{_, _, max u₁ u₂ u₃ w} Semantics.Empty V m n
   := (proc.semantics.guard opSpec.TrivGuard).interpret opInterp
 
+theorem compile_forward_sim_guarded
+  [Arity Op] [PCM T] [PCM.Lawful T]
+  [DecidableEq χ]
+  [InterpConsts V]
+  {sigs : Sigs k}
+  {opSpec : OpSpec Op V T}
+  {progSpec : ProgSpec Op V T sigs}
+  (prog : ProgWithSpec χ sigs opSpec)
+  (hwt : ProgWithSpec.WellPermTyped progSpec prog)
+  (haff₁ : ∀ i, (prog i).AffineVar)
+  (haff₂ : prog.AffineInrOp)
+  (i : Fin k) :
+    (prog.semantics i).guard opSpec.TrivGuard
+      ≲ᵣ (compileProg prog i).semantics.guard (opSpec.Guard (progSpec i))
+  := by
+  apply IORestrictedSimilarity.trans
+  · exact sim_wt_prog prog hwt
+  apply sim_guard
+  apply sim_compile_prog prog i haff₁ haff₂
+
 theorem compile_forward_sim
   [Arity Op] [PCM T] [PCM.Lawful T]
   [DecidableEq χ]
@@ -74,22 +94,23 @@ theorem compile_forward_sim
       ≲ᵣ (compileProg prog i).semantics.guard opSpec.TrivGuard
   := by
   apply IORestrictedSimilarity.trans
-  · exact sim_wt_prog prog hwt
-  apply IORestrictedSimilarity.trans
-  · apply sim_guard
-    apply sim_compile_prog prog i haff₁ haff₂
-  simp
+  · apply compile_forward_sim_guarded prog hwt haff₁ haff₂ i
   sorry
 
 theorem compile_strong_norm
   {Op V T : Type u}
-  [Arity Op] [PCM T] [PCM.Lawful T]
+  [Arity Op] [PCM T] [PCM.Lawful T] [PCM.Cancellative T]
   [DecidableEq χ]
   [InterpConsts V]
   [opInterp : OpInterp.{_, _, w} Op V]
   {sigs : Sigs k}
   {opSpec : OpSpec Op V T}
   {progSpec : ProgSpec Op V T sigs}
+
+  (hconfl : opSpec.Confluent opInterp)
+  (hdet : opInterp.Deterministic)
+  (hnb : opInterp.NonBlocking)
+
   (prog : Prog (WithSpec Op opSpec) χ (V ⊕ T) (extendSigs sigs))
   (hwt : ProgWithSpec.WellPermTyped progSpec prog)
   (haff₁ : ∀ (i : Fin k), (prog i).AffineVar)
@@ -103,23 +124,100 @@ theorem compile_strong_norm
 
   {s s₁ s₂ : (prog.semanticsᵢ i).S}
   {s' s₁' : proc.semanticsᵢ.S}
-  -- Same input values to both semantics
-  (hinputs : (prog.semanticsᵢ i).lts.Step (prog.semanticsᵢ i).init (.input args) s)
-  (hinputs' : proc.semanticsᵢ.lts.Step proc.semanticsᵢ.init (.input args) s')
 
   -- There exists a terminating trace in the sequential semantics
   -- that output `outputVals`.
+  (hinputs : (prog.semanticsᵢ i).lts.Step (prog.semanticsᵢ i).init (.input args) s)
   (htrace : (prog.semanticsᵢ i).lts.TauStarN .τ k s s₁)
   (hterm : (prog.semanticsᵢ i).lts.IsFinalFor (·.isSilent) s₁)
   (houtput : (prog.semanticsᵢ i).lts.Step s₁ (.output outputVals) s₂)
 
+  (hinputs' : proc.semanticsᵢ.lts.Step proc.semanticsᵢ.init (.input args) s')
   (htrace' : proc.semanticsᵢ.lts.TauStarN .τ k' s' s₁') :
     ∃ (s₁'' s₂' : proc.semanticsᵢ.S) (k'' : Nat),
-      k = k' + k'' ∧
+      -- k = k' + k'' ∧
       proc.semanticsᵢ.lts.TauStarN .τ k'' s₁' s₁'' ∧
       proc.semanticsᵢ.lts.IsFinalFor (·.isSilent) s₁'' ∧
       proc.semanticsᵢ.lts.Step s₁'' (.output outputVals) s₂' ∧
       s₂'.2 = s₂.2 -- Equal "memory" states
-  := sorry
+  := by
+  /- Sketch
+  Notations:
+    - →ι : input step
+    - →τ : silent step
+    - →ω : output step
+    - ∼ : suitable simulation relation
+
+  We have:
+    `Seq`: init →ι s →τ* s₁ →ω s₂, (s₁ final wrt to τ)
+    `Proc`: init →ι s' →τ* s₁'
+
+  By simulation, we get
+    `Proc`: init →ι s'' →τ* s''', with s''' ∼ s₁
+    `Proc`: s''' →τ* s₁'', with s₁'' ∼ s₁
+    `Proc`: s₁'' →τ* s₁''' →ω s₂'', with s₂'' ∼ s₂
+    In other words:
+      init →ι s'' →τ* s₁''' →ω s₂'', with s₂'' ∼ s₂
+
+  TODO
+  -/
+  subst hcomp
+  have hsim₁ := compile_forward_sim_guarded prog hwt haff₁ haff₂ i
+  replace hsim₁ := sim_interp hsim₁
+  -- Carry the first input step over
+  have ⟨s''', hinputs'', hsim_s'''⟩ := hsim₁.sim_step _ _ _ _ hsim₁.sim_init hinputs
+  cases hinputs'' with | step_input hinputs'' htau₁ =>
+  rename_i s''
+  have heq₁ := proc_interp_guarded_unguarded_det_input_mod hinputs'' hinputs'
+  -- Carry the silent steps after the first input steps
+  have := congr_eq_mod_ghost_proc_interp_unguarded_tau_star_n htrace'
+    (by
+      constructor
+      · exact IsSymm.symm _ _ heq₁.1
+      · exact heq₁.2.symm)
+  have ⟨_, htrace'', heq₂⟩ := this
+  -- Carry the middle τ* steps over
+  have ⟨s₁'', hstep_s₁'', hsim_s₁''⟩ := hsim₁.map_tau_star hsim_s''' htrace.without_length
+  -- Carry the final output step over
+  have ⟨s₂'', houtput', hsim_s₂''⟩ := hsim₁.sim_step _ _ _ _ hsim_s₁'' houtput
+  cases houtput' with | step_output htau₂ houtput' =>
+  rename_i s₁'''
+  -- Concatenate the middle steps in guarded proc semantics
+  have hmiddle := (htau₁.trans hstep_s₁'').trans htau₂
+  replace ⟨k', hmiddle⟩ := hmiddle.with_length
+  -- have hfinal_s₁''' :
+  -- Use determinacy
+  have ⟨_, _, htrace''', hlen₁, heq₃⟩ := proc_interp_guarded_hetero_terminal_confl hconfl hdet hnb
+    sorry sorry hmiddle sorry htrace''
+  -- Convert the determinacy result to τ steps after `htrace'`
+  have this := congr_eq_mod_ghost_proc_interp_unguarded_tau_star_n htrace'''
+    (by
+      constructor
+      · exact IsSymm.symm _ _ heq₂.1
+      · exact heq₂.2.symm)
+  have ⟨s₁'''', htrace'''', heq₄⟩ := this
+  -- Carry the final output step over through ≈
+  have houtput'' := Config.InterpGuardStep.to_indexed_interp_unguarded houtput'
+  have ⟨_, houtput''', _⟩ := congr_eq_mod_ghost_proc_interp_unguarded_output
+    (s₁' := s₁'''')
+    houtput'' (by
+      constructor
+      · trans
+        · exact heq₃.1
+        · exact heq₄.1
+      · simp [heq₃.2, heq₄.2])
+  -- have := htrace'.trans htrace''''
+  exact ⟨
+    _, _, _, htrace'''',
+    sorry,
+    houtput''',
+    by
+      -- The final output step does not change the shared operator state
+      simp [← houtput'''.output_eq_state,
+        ← houtput.output_eq_state]
+      simp [← heq₄.2, ← heq₃.2, houtput'.output_eq_state]
+      -- TODO: infer from hsim_s₂'' the final equality
+      sorry
+  ⟩
 
 end Wavelet
