Wavelet/Semantics/Defs.lean
@@ -453,6 +453,17 @@ theorem IORestrictedSimilarity.to_weak_sim
       | step_tau htau => exact .from_tau_star htau
     · exact hR'
 
+theorem IORestrictedSimilarity.map_tau_star
+  [Arity Op]
+  {sem₁ sem₂ : Semantics Op V m n}
+  (hsim : sem₁ ≲ᵣ sem₂)
+  {s₁ s₁' : sem₁.S}
+  {s₂ : sem₂.S}
+  (h : hsim.Sim s₁ s₂)
+  (htau : sem₁.lts.TauStar .τ s₁ s₁') :
+    ∃ s₂', sem₂.lts.TauStar .τ s₂ s₂' ∧ hsim.Sim s₁' s₂'
+  := sorry
+
 instance [Arity Op] : IsRefl (Semantics Op V m n) IORestrictedSimilarity where
   refl := .refl
 
